proved correction of union

proofs/joinWB.v
@@ -1,5 +1,5 @@
 From Hammer Require Import Tactics.
-From BalancedTrees Require Import definitions utils.
+From BalancedTrees Require Import definitions utils trees.
 From AAC_tactics Require Import AAC.
 From AAC_tactics Require Import Instances.
 Import Lists.
@@ -289,10 +289,223 @@ Proof.
       intuition aac_rewrite H9; aac_reflexivity.
 Qed.
 
-Lemma joinWB : forall T__L k T__R, WB T__L -> WB T__R -> WB (join T__L k T__R) /\ elements (join T__L k T__R) =  elements (Node T__L k T__R).
+Theorem join_correct : forall T__L k T__R, WB T__L -> WB T__R -> WB (join T__L k T__R) /\ elements (join T__L k T__R) =  elements (Node T__L k T__R).
 Proof.
   intros. unfold join. remember (not_left_heavyb (weight T__L) (weight T__R)) as b; destruct b.
   - apply join_maybe_right_heavyWB; auto. rewrite not_left_heavy_equiv. auto.
   - apply join_maybe_left_heavyWB; auto. apply eq_sym in Heqb. rewrite  <- not_left_heavy_equiv_false in Heqb.
     unfold not_right_heavy, not_left_heavy, alpha in *. remember (weight_ge_one T__R). lia.
+Qed.
+
+Lemma joinWB : forall T__L k T__R, WB T__L -> WB T__R -> WB (join T__L k T__R).
+Proof.
+  apply join_correct.
+Qed.
+
+Lemma join_elts : forall T__L k T__R, WB T__L -> WB T__R -> elements (join T__L k T__R) = elements (Node T__L k T__R).
+Proof.
+  apply join_correct.
+Qed.
+
+Lemma join_occurs : forall T__L k T__R x, WB T__L -> WB T__R -> x ∈ join T__L k T__R <-> x ∈ T__L \/ x = k \/ x ∈ T__R.
+Proof.
+  unfold occurs. intros. rewrite join_elts; auto.
+  change ((x ∈ elements ?a)%stdpp) with (occurs x a). intuition. apply occurs_rec in H1.
+  intuition auto.
+Qed.
+
+Lemma join_abr : forall T__L k T__R, WB T__L -> WB T__R -> abr T__L -> abr T__R -> all_smallers T__L k ->
+                            all_greaters T__R k -> abr (join T__L k T__R).
+Proof.
+  intros. unfold abr. rewrite join_elts; auto. apply abr_node. tauto.
+Qed.
+
+Close Scope Z_scope.
+
+Equations split (T: Tree) (k: A) : Tree * bool * Tree :=
+| Leaf, _ => (Leaf, false, Leaf)
+| Node l k' r, k with k ?= k' => {
+  | Eq => (l, true, r)
+  | Lt with split l k => {
+    | (ll, b, lr) => (ll, b, join lr k' r)
+    }
+  | Gt with split r k => {
+    | (rl, b, rr) => (join l k' rl, b, rr)
+    }
+  }.
+
+Lemma splitWB : forall T k a b c, WB T -> split T k = (a, b, c) -> WB a /\ WB c.
+Proof.
+  intros T k. funelim (split T k).
+  - simp split. auto.
+  - rewrite <- Heqcall. intros. inversion H0. subst. inversion H. auto.
+  - rewrite <- Heqcall. intros. inversion H0. subst. specialize (Hind a b0 lr). inversion H.
+    subst. intuition auto. apply joinWB; auto.
+  - rewrite <- Heqcall. intros. inversion H0. subst. specialize (Hind rl b0 c). inversion H.
+    subst. intuition auto. apply joinWB; auto.
+Qed.
+
+Lemma split_b : forall T k a b c, WB T -> abr T -> split T k = (a, b, c) -> b = occursb k T.
+Proof.
+  intros T k. funelim (split T k).
+  - simp split. auto.
+  - rewrite <- Heqcall. apply Nat.compare_eq in Heq. subst. intros. inversion H1. subst.
+    apply eq_sym. rewrite occursb_correct. auto.
+  - rewrite <- Heqcall. intros. inversion H1. subst. inversion H. subst.
+    apply abr_node in H0 as Habrs. intuition.
+    specialize (Hind _ _ _ H5 H2 Heq). subst.
+    enough (occursb k l = true <-> occursb k (Node l k' r) = true).
+    + destruct (occursb k l); destruct (occursb k (Node l k' r)); intuition congruence.
+    + repeat rewrite occursb_correct. intuition auto. eapply abr_lt_occurs; eauto.
+      apply Nat.compare_lt_iff. auto.
+  - rewrite <- Heqcall. intros. inversion H1. subst. inversion H. subst.
+    apply abr_node in H0 as Habrs. intuition.
+    specialize (Hind _ _ _ H6 H4 Heq). subst.
+    enough (occursb k r = true <-> occursb k (Node l k' r) = true).
+    + destruct (occursb k r); destruct (occursb k (Node l k' r)); intuition congruence.
+    + repeat rewrite occursb_correct. intuition auto. eapply abr_gt_occurs; eauto.
+      apply Nat.compare_gt_iff. auto.
+Qed.
+
+Lemma split_elts_occursb : forall T k a b c,
+    WB T -> abr T -> split T k = (a, b, c) ->
+    elements T = elements a ++ delta (occursb k T) k ++ elements c.
+Proof.
+  intros T k. funelim (split T k).
+  - simp split. auto.
+  - rewrite <- Heqcall. apply Nat.compare_eq in Heq. subst. intros. inversion H1. subst.
+    simp elements. repeat f_equal. assert (occursb k' (Node a k' c) = true).
+    + apply occursb_correct. auto.
+    + rewrite H2. auto.
+  - rewrite <- Heqcall. intros. apply abr_node in H0 as Habr. inversion H. subst. intuition.
+    specialize (Hind _ _ _ H5 H2 Heq).
+    apply split_b in Heq as Heq'; auto. apply eq_sym in Heq'. rewrite Heq' in *. destruct b.
+    + assert (occursb k (Node l k' r) = true).
+      * rewrite occursb_correct in *. apply occurs_rec. auto.
+      * rewrite H8. inversion H1. subst.
+        apply splitWB in Heq as Heq2; auto. intuition. rewrite join_elts; auto. simp elements.
+        rewrite Hind. aac_reflexivity.
+    + assert (~ occurs k (Node l k' r)).
+      * intro. apply Nat.compare_lt_iff in Heq0. apply abr_lt_occurs in H8; auto.
+        apply occursb_correct in H8. congruence.
+      * rewrite <- occursb_correct in H8. apply not_true_is_false in H8. rewrite H8.
+        simp elements. rewrite Hind. inversion H1. subst. apply splitWB in Heq; auto. intuition.
+        rewrite join_elts; auto. simp elements. aac_reflexivity.
+  - rewrite <- Heqcall. intros. apply abr_node in H0 as Habr. inversion H. subst. intuition.
+    specialize (Hind _ _ _ H6 H4 Heq).
+    apply split_b in Heq as Heq'; auto. apply eq_sym in Heq'. rewrite Heq' in *. destruct b.
+    + assert (occursb k (Node l k' r) = true).
+      * rewrite occursb_correct in *. apply occurs_rec. auto.
+      * rewrite H8. inversion H1. subst.
+        apply splitWB in Heq as Heq2; auto. intuition. rewrite join_elts; auto. simp elements.
+        rewrite Hind. aac_reflexivity.
+    + assert (~ occurs k (Node l k' r)).
+      * intro. apply Nat.compare_gt_iff in Heq0. apply abr_gt_occurs in H8; auto.
+        apply occursb_correct in H8. congruence.
+      * rewrite <- occursb_correct in H8. apply not_true_is_false in H8. rewrite H8.
+        simp elements. rewrite Hind. inversion H1. subst. apply splitWB in Heq; auto. intuition.
+        rewrite join_elts; auto. simp elements. aac_reflexivity.
+Qed.
+
+Lemma split_occurs : forall T k a b c,
+    WB T -> abr T -> split T k = (a, b, c) -> forall x, x ∈ a \/ x ∈ c -> x ∈ T.
+Proof.
+  unfold occurs. intros. rewrite (split_elts_occursb _ _ _ _ _ H H0 H1).
+  repeat rewrite elem_of_app. intuition auto.
+Qed.
+
+Lemma split_occurs_recipr : forall T k a b c,
+    WB T -> abr T -> split T k = (a, b, c) -> forall x, x ∈ T -> x ∈ a \/ x ∈ c \/ (x = k /\ b = true).
+Proof.
+  unfold occurs. intros.
+  rewrite (split_elts_occursb _ _ _ _ _ H H0 H1), elem_of_app, elem_of_app in H2.
+  intuition auto. apply split_b, eq_sym in H1; auto.  destruct b.
+  - rewrite H1 in *. simpl delta in *. apply elem_of_list_singleton in H2.
+    subst. auto.
+  - rewrite H1 in *. simpl delta in *. inversion H2.
+Qed.
+
+Lemma split_abr : forall T k a b c,
+    WB T -> abr T -> split T k = (a, b, c) -> abr a /\ abr c.
+Proof.
+  intros. apply split_elts_occursb in H1; auto. unfold abr in *. rewrite H1 in *.
+  eauto using StronglySorted_app_inv_l, StronglySorted_app_inv_r.
+Qed.
+
+Lemma split_smallers_greaters : forall T k a b c,
+    WB T -> abr T -> split T k = (a, b, c) -> all_smallers a k /\ all_greaters c k.
+Proof.
+  intros T k. funelim (split T k).
+  - simp split. intros. unfold all_smallers, all_greaters. inversion H1. subst. simp elements.
+    auto.
+  - apply Nat.compare_eq in Heq. subst. rewrite <- Heqcall. intros. apply abr_node in H0.
+    inversion H1. subst. tauto.
+  - rewrite <- Heqcall. intros. inversion H. subst. apply abr_node in H0 as Habr. inversion H1.
+    subst. destruct Habr. specialize (Hind _ _ _ H5 H2 Heq). intuition.
+    unfold all_greaters. apply splitWB in Heq as Heq'; auto. rewrite join_elts; try tauto.
+    simp elements. apply List.Forall_app. intuition. apply List.Forall_app.
+    apply Nat.compare_lt_iff in Heq0. intuition. eapply greater_trans; eauto.
+  - rewrite <- Heqcall. intros. inversion H. subst. apply abr_node in H0 as Habr. inversion H1.
+    subst. destruct Habr. destruct H3. specialize (Hind _ _ _ H6 H3 Heq). intuition.
+    unfold all_smallers. apply splitWB in Heq as Heq'; auto. rewrite join_elts; try tauto.
+    simp elements. apply List.Forall_app. apply Nat.compare_gt_iff in Heq0. intuition.
+    { eapply smaller_trans; eauto. }
+    apply List.Forall_app. auto.
+Qed.
+
+Equations union (T1 T2: Tree) : Tree :=
+| Leaf, T2 => T2
+| T1, Leaf => T1
+| T1, Node L2 k R2 with split T1 k => {
+  | (L1, _, R1) => join (union L1 L2) k (union R1 R2)
+  }.
+
+Lemma unionWB : forall T1 T2, WB T1 -> WB T2 -> WB (union T1 T2).
+Proof.
+  intros. funelim (union T1 T2).
+  - rewrite <- Heqcall. auto.
+  - simp union.
+  - rewrite <- Heqcall. inversion H2. subst. apply splitWB in Heq; auto. destruct Heq.
+    intuition. apply joinWB; auto.
+Qed.
+
+Lemma union_keeps_elts : forall T1 T2 x,
+    WB T1 -> WB T2 -> abr T1 -> abr T2 -> x ∈ union T1 T2 <-> x ∈ T1 \/ x ∈ T2.
+Proof.
+  intros. funelim (union T1 T2).
+  - rewrite <- Heqcall. intuition auto. inversion H4.
+  - simp union. intuition auto. inversion H4.
+  - rewrite <- Heqcall. clear Heqcall. apply splitWB in Heq as Heq'; auto. destruct Heq'.
+    inversion H2. subst. remember unionWB. rewrite join_occurs; auto.
+    apply abr_node in H3 as Habr1. apply abr_node in H4 as Habr2.
+    apply split_abr in Heq as Heq'; auto.
+    rewrite H; try tauto. rewrite H0; try tauto. intuition eauto using split_occurs.
+    + apply occurs_rec in H21.
+      intuition apply split_occurs_recipr with (x := x) in Heq; intuition auto.
+    + apply occurs_rec in H21. intuition auto. 
+Qed.
+
+Lemma union_keeps_abr : forall T1 T2, WB T1 -> WB T2 -> abr T1 -> abr T2 -> abr (union T1 T2).
+Proof.
+  intros. funelim (union T1 T2).
+  - rewrite <- Heqcall. auto.
+  - simp union.
+  - rewrite <- Heqcall. inversion H1. inversion H2. apply splitWB in Heq as Heq'; intuition.
+    subst. apply split_abr in Heq as Heq'; intuition auto. apply abr_node in H4. intuition.
+    apply join_abr; auto using unionWB.
+    + unfold all_smallers. rewrite Forall_forall. intro. pose union_keeps_elts.
+      unfold occurs in i. rewrite i; auto. intro Hocc.
+      destruct Hocc as [ Hocc | Hocc ]; revert Hocc; generalize x; apply Forall_forall; auto.
+      eapply split_smallers_greaters; try eexact Heq; eauto.
+    + unfold all_greaters. rewrite Forall_forall. intro. pose union_keeps_elts.
+      unfold occurs in i. rewrite i; auto. intro Hocc.
+      destruct Hocc as [ Hocc | Hocc ]; revert Hocc; generalize x; apply Forall_forall; auto.
+      eapply split_smallers_greaters; try eexact Heq; eauto.
+Qed.
+
+Theorem union_works : forall T1 T2,
+    abr T1 -> abr T2 -> WB T1 -> WB T2 ->
+    WB (union T1 T2) /\ abr (union T1 T2) /\ (forall x, x ∈ union T1 T2 <-> x ∈ T1 \/ x ∈ T2).
+Proof.
+  intuition auto using unionWB, union_keeps_abr; apply union_keeps_elts; auto.
 Qed.
